Separate recovery correctness and idempotence
Idempotence turns out to be tricky due to how ghost state is handled,
and due to an imprecision in the current fixup/recovery specs: we need a
guarantee that if the precondition is in the state where the disks are
equal, the postcondition will not have diskUpd (a more precise
combination of the three separate proofs for fixup that cover all the
input cases).

src/Shallow/ProgLang/Hoare.v
@@ -151,17 +151,23 @@ Proof.
   eapply H; eauto.
 Qed.
 
+Definition spec_impl
+           `(spec1: Specification A' T State)
+           `(spec2: Specification A T State) :=
+  forall a state, pre (spec2 a state) ->
+         exists a', pre (spec1 a' state) /\
+               (forall v state', post (spec1 a' state) v state' ->
+                        post (spec2 a state) v state') /\
+               (forall state', crash (spec1 a' state) state' ->
+                      crash (spec2 a state) state').
+
+
 Theorem spec_weaken : forall `(step: Semantics opT State)
                         `(spec1: Specification A' T State)
                         `(spec2: Specification A T State)
                         (p: prog opT T),
     prog_spec spec1 p step ->
-    forall (Himpl: forall a state, pre (spec2 a state) ->
-                      exists a', pre (spec1 a' state) /\
-                           (forall v state', post (spec1 a' state) v state' ->
-                                    post (spec2 a state) v state') /\
-                           (forall state', crash (spec1 a' state) state' ->
-                                  crash (spec2 a state) state')),
+    forall (Himpl: spec_impl spec1 spec2),
       prog_spec spec2 p step.
 Proof.
   unfold prog_spec; intros.
